coq/handwritten/Lift/Lift/ConnectionLift.v
@@ -1,0 +1,554 @@
+From Coq Require Import Vectors.Vector.
+From Coq Require Import ssreflect.
+
+From mathcomp Require Import eqtype.
+From mathcomp Require Import ssrfun.
+From mathcomp Require Import ssrnat.
+
+From CryptolToCoq Require Import CryptolPrimitivesForSAWCore.
+From CryptolToCoq Require Import CryptolPrimitivesForSAWCoreExtra.
+From CryptolToCoq Require Import SAWCorePrelude.
+From CryptolToCoq Require Import SAWCorePrelude_proofs.
+From CryptolToCoq Require Import SAWCoreScaffolding.
+From CryptolToCoq Require Import SAWCoreVectorsAsCoqVectors.
+
+From Lift Require Import Preprocess.S2NPP.
+From Lift Require Import Preprocess.HandshakePP.
+From Lift Require Import Preprocess.ConnectionPP.
+
+From Lift Require Import Lift.HandshakeLift.
+
+From Ornamental Require Import Ornaments.
+
+From S2N Require Import S2N.
+
+Set DEVOID search prove equivalence.
+Set DEVOID lift type.
+
+Import CryptolPrimitives.
+
+Module ConnectionAccessors.
+
+  Definition get_client_auth_flag (c : Connection.connection) : bool :=
+    fst c.
+
+  Definition get_corked (c : Connection.connection) : seq 2 bool :=
+    fst (snd c).
+
+  Definition get_corked_IO (c : Connection.connection) : seq 8 bool :=
+    fst (snd (snd c)).
+
+  Definition get_handshake (c : Connection.connection) : Handshake.handshake :=
+    fst (snd (snd (snd c))).
+
+  (* Definition get_is_caching_enabled (c : connection) : bool := *)
+  (*   fst (snd (snd (snd (snd c)))). *)
+
+  (* Definition get_key_exchange_EPH (c : connection) : bool := *)
+  (*   fst (snd (snd (snd (snd (snd c))))). *)
+
+  (* Definition get_mode (c : connection) : seq 32 bool := *)
+  (*   fst (snd (snd (snd (snd (snd (snd c)))))). *)
+
+  (* Definition get_resume_from_cache (c : connection) : bool := *)
+  (*   fst (snd (snd (snd (snd (snd (snd (snd c))))))). *)
+
+  (* Definition get_server_can_send_ocsp (c : connection) : bool := *)
+  (*   snd (snd (snd (snd (snd (snd (snd (snd c))))))). *)
+
+End ConnectionAccessors.
+
+Module ConnectionRecord.
+
+  Record Connection :=
+    MkConnection
+      {
+        clientAuthFlag    : bool;
+        corked            : seq 2 bool;
+        corkedIO          : seq 8 bool;
+        handshake         : HandshakeRecordPP.Handshake;
+        isCachingEnabled  : bool;
+        keyExchangeEPH    : bool;
+        mode              : seq 32 bool;
+        resumeFromCache   : bool;
+        serverCanSendOCSP : bool;
+      }.
+
+  Scheme Induction for Connection Sort Prop.
+  Scheme Induction for Connection Sort Type.
+  Scheme Induction for Connection Sort Set.
+
+End ConnectionRecord.
+
+Preprocess Module ConnectionAccessors
+  as ConnectionAccessorsPP
+       { opaque
+           Handshake.handshake
+           fst snd
+           natToNat
+           seq
+     }.
+
+Preprocess Module ConnectionRecord
+  as ConnectionRecordPP0
+       { opaque
+           Handshake.handshake
+           fst snd
+           natToNat
+           seq
+     }.
+
+Lift Module
+     HandshakePP.handshake
+     HandshakeRecordPP.Handshake
+  in ConnectionRecordPP0
+  as ConnectionRecordPP1.
+
+(* We need to be able to talk about the type that is just like ConnectionPP.connection, but with *)
+(* HandshakePP.handshake replaced with HandshakeRecordPP.Handhake. *)
+Lift Handshake.handshake
+     HandshakeRecordPP.Handshake
+  in ConnectionPP.connection
+  as ConnectionPPconnection.
+
+Lift Module
+     ConnectionPPconnection
+     ConnectionRecordPP1.Connection
+  in ConnectionRecordPP1
+  as ConnectionRecordPP.
+
+Lift HandshakePP.handshake
+     HandshakeRecordPP.Handshake
+  in S2N'.s2n_cork
+  as s2nCork0
+       { opaque ecPlus PArithSeqBool ecNumber PLiteralSeqBool
+       }.
+
+Lift ConnectionPPconnection
+     ConnectionRecordPP0.Connection
+  in s2nCork0
+  as s2nCork
+       { opaque ecPlus PArithSeqBool ecNumber PLiteralSeqBool
+       }.
+
+Lift HandshakePP.handshake
+     HandshakeRecordPP.Handshake
+  in S2N'.s2n_uncork
+  as s2nUncork0
+       { opaque ecMinus PArithSeqBool ecNumber PLiteralSeqBool
+       }.
+
+Lift ConnectionPPconnection
+     ConnectionRecordPP0.Connection
+  in s2nUncork0
+  as s2nUncork
+       { opaque ecMinus PArithSeqBool ecNumber PLiteralSeqBool
+       }.
+
+Definition cork (c : ConnectionRecordPP0.Connection) : ConnectionRecordPP0.Connection :=
+  {|
+  ConnectionRecordPP0.clientAuthFlag    := ConnectionRecordPP0.clientAuthFlag c;
+  ConnectionRecordPP0.corked            := s2nCork c;
+  ConnectionRecordPP0.corkedIO          := ConnectionRecordPP0.corkedIO c;
+  ConnectionRecordPP0.handshake         := ConnectionRecordPP0.handshake c;
+  ConnectionRecordPP0.isCachingEnabled  := ConnectionRecordPP0.isCachingEnabled c;
+  ConnectionRecordPP0.keyExchangeEPH    := ConnectionRecordPP0.keyExchangeEPH c;
+  ConnectionRecordPP0.mode              := ConnectionRecordPP0.mode c;
+  ConnectionRecordPP0.resumeFromCache   := ConnectionRecordPP0.resumeFromCache c;
+  ConnectionRecordPP0.serverCanSendOCSP := ConnectionRecordPP0.serverCanSendOCSP c;
+  |}.
+
+Definition uncork (c : ConnectionRecordPP0.Connection) : ConnectionRecordPP0.Connection :=
+  {|
+  ConnectionRecordPP0.clientAuthFlag    := ConnectionRecordPP0.clientAuthFlag c;
+  ConnectionRecordPP0.corked            := s2nUncork c;
+  ConnectionRecordPP0.corkedIO          := ConnectionRecordPP0.corkedIO c;
+  ConnectionRecordPP0.handshake         := ConnectionRecordPP0.handshake c;
+  ConnectionRecordPP0.isCachingEnabled  := ConnectionRecordPP0.isCachingEnabled c;
+  ConnectionRecordPP0.keyExchangeEPH    := ConnectionRecordPP0.keyExchangeEPH c;
+  ConnectionRecordPP0.mode              := ConnectionRecordPP0.mode c;
+  ConnectionRecordPP0.resumeFromCache   := ConnectionRecordPP0.resumeFromCache c;
+  ConnectionRecordPP0.serverCanSendOCSP := ConnectionRecordPP0.serverCanSendOCSP c;
+  |}.
+
+Module CorkTheoremLow.
+
+  Definition justCork
+             (b : bool) (s0 : seq 8 bool) (h : Handshake.handshake) (b0 b1 : bool) (s1 : seq 32 bool) (b2 b3 : bool) :=
+      S2N'.s2n_cork (b, (joinLSB (joinLSB (nil bool) false) false, (s0, (h, (b0, (b1, (s1, (b2, b3)))))))).
+
+  Definition lemma_1_type :=
+    forall (b : bool) (s0 : seq 8 bool) (h : Handshake.handshake) (b0 b1 : bool) (s1 : seq 32 bool) (b2 b3 : bool),
+      S2N'.s2n_cork (b, (joinLSB (joinLSB (nil bool) false) false, (s0, (h, (b0, (b1, (s1, (b2, b3)))))))) =
+      joinLSB (joinLSB (nil bool) false) true.
+
+  Lemma lemma_1 : lemma_1_type.
+  Proof.
+    intros b s0 h b0 b1 s1 b2 b3.
+    unfold S2N'.s2n_cork.
+    simpl.
+    unfold ecPlus; simpl.
+    unfold Notation.Rget; simpl.
+    unfold bvAdd; simpl.
+    unfold joinLSB; simpl.
+    reflexivity.
+  Defined.
+
+  Theorem cork_theorem_low : forall c,
+    ConnectionAccessors.get_corked c = bvNat 2 0 ->
+    S2N'.s2n_cork c = bvNat 2 1.
+  Proof.
+    intros [? [? [? [? [? [? [? [? ?]]]]]]]].
+    simpl.
+    unfold ConnectionAccessors.get_corked.
+    simpl.
+    intros.
+    subst s.
+    apply lemma_1.
+  Defined.
+
+End CorkTheoremLow.
+
+Set Preprocess default opaque.
+
+Preprocess
+  Module CorkTheoremLow
+  as CorkTheoremLowPP.
+
+Lift HandshakePP.handshake
+     HandshakeRecordPP.Handshake
+  in CorkTheoremLowPP.justCork
+  as CorkTheoremLow_justCork0
+       { opaque joinLSB
+       }.
+
+(* From Ornamental Require Import Patcher.Patch. *)
+
+Definition two := 2.
+Definition eight := 8.
+Definition thirtyTwo := 32.
+
+From Patcher Require Import Patch.
+
+Replace Convertible Module
+        two eight thirtyTwo
+  in CorkTheoremLowPP
+  as CorkTheoremLowPP'.
+
+Print CorkTheoremLowPP'.lemma_1.
+
+Lift HandshakePP.handshake
+     HandshakeRecordPP.Handshake
+  in CorkTheoremLowPP'.lemma_1_type
+  as CorkTheoremLow_lemma_1_type_0.
+
+Check (CorkTheoremLowPP'.lemma_1 : CorkTheoremLowPP'.lemma_1_type).
+
+Lift HandshakePP.handshake
+     HandshakeRecordPP.Handshake
+  in CorkTheoremLowPP'.lemma_1
+  as CorkTheoremLow_lemma_1_0
+       { opaque
+
+           Ascii.Ascii
+           BinNums.xI
+           BinNums.xO
+           Bool
+           CoreRecords.FScons
+           CoreRecords.field
+           CoreRecords.Fields
+           CoreRecords.get_member
+           CoreRecords.pm_Branch
+           CoreRecords.pm_Leaf
+           CoreRecords.record_get
+           CoreRecords.string_to_p
+           Datatypes.snd
+           Logic.eq_refl
+           Notation.Rget
+           PArithWord
+           PLiteralSeqBool
+           String.EmptyString
+           String.String
+           TCNum
+           bitvector
+           bool
+           bvAdd
+           bvNat
+           bvToBITS
+           cons
+           ecNumber
+           ecPlus
+           eight
+           half
+           joinLSB
+           nil
+           odd
+           operations.adcB
+           prod
+           seq
+           shiftin
+           spec.BITS
+           spec.toNat
+           thirtyTwo
+           two
+
+           (* those should probably be transparent in the real one *)
+           (* S2N'.s2n_cork *)
+           (* prod *)
+
+       }.
+
+Lift HandshakePP.handshake
+     HandshakeRecordPP.Handshake
+  in CorkTheoremLowPP'.cork_theorem_low
+  as CorkTheoremLow_cork_theorem_low_0
+       { opaque
+
+           Ascii.Ascii
+           BinNums.xI
+           BinNums.xO
+           Bool
+           CoreRecords.FScons
+           CoreRecords.field
+           CoreRecords.Fields
+           CoreRecords.get_member
+           CoreRecords.pm_Branch
+           CoreRecords.pm_Leaf
+           CoreRecords.record_get
+           CoreRecords.string_to_p
+           Datatypes.snd
+           Logic.eq_refl
+           Notation.Rget
+           PArithWord
+           PLiteralSeqBool
+           String.EmptyString
+           String.String
+           TCNum
+           bitvector
+           bool
+           bvAdd
+           bvNat
+           bvToBITS
+           cons
+           ecNumber
+           ecPlus
+           eight
+           half
+           joinLSB
+           nil
+           odd
+           operations.adcB
+           prod
+           seq
+           shiftin
+           spec.BITS
+           spec.toNat
+           thirtyTwo
+           two
+
+           (* those should probably be transparent in the real one *)
+           (* S2N'.s2n_cork *)
+           (* prod *)
+
+       }.
+
+Lift ConnectionPPconnection
+     ConnectionRecordPP0.Connection
+  in CorkTheoremLow_lemma_1_type_0
+  as CorkTheoremLow_lemma_1_type_1.
+
+Lift ConnectionPPconnection
+     ConnectionRecordPP0.Connection
+  in CorkTheoremLow_lemma_1_0
+  as CorkTheoremLow_lemma_1_1
+       { opaque
+
+           Ascii.Ascii
+           BinNums.xI
+           BinNums.xO
+           Bool
+           CoreRecords.FScons
+           CoreRecords.field
+           CoreRecords.Fields
+           CoreRecords.get_member
+           CoreRecords.pm_Branch
+           CoreRecords.pm_Leaf
+           CoreRecords.record_get
+           CoreRecords.string_to_p
+           Datatypes.snd
+           Logic.eq_refl
+           Notation.Rget
+           PArithWord
+           PLiteralSeqBool
+           String.EmptyString
+           String.String
+           TCNum
+           bitvector
+           bool
+           bvAdd
+           bvNat
+           bvToBITS
+           cons
+           ecNumber
+           ecPlus
+           eight
+           half
+           joinLSB
+           nil
+           odd
+           operations.adcB
+           prod
+           seq
+           shiftin
+           spec.BITS
+           spec.toNat
+           thirtyTwo
+           two
+
+           (* those should probably be transparent in the real one *)
+           (* S2N'.s2n_cork *)
+           (* prod *)
+
+       }.
+
+(* STUCK *)
+
+Lift ConnectionPPconnection
+     ConnectionRecordPP0.Connection
+  in CorkTheoremLow_cork_theorem_low_0
+  as CorkTheoremLow_cork_theorem_low_1
+       { opaque
+
+           Ascii.Ascii
+           BinNums.xI
+           BinNums.xO
+           Bool
+           CoreRecords.FScons
+           CoreRecords.field
+           CoreRecords.Fields
+           CoreRecords.get_member
+           CoreRecords.pm_Branch
+           CoreRecords.pm_Leaf
+           CoreRecords.record_get
+           CoreRecords.string_to_p
+           Logic.eq_refl
+           Notation.Rget
+           PArithWord
+           PLiteralSeqBool
+           String.EmptyString
+           String.String
+           TCNum
+           bitvector
+           bool
+           bvAdd
+           bvNat
+           bvToBITS
+           cons
+           ecNumber
+           ecPlus
+           eight
+           half
+           joinLSB
+           nil
+           odd
+           operations.adcB
+           seq
+           shiftin
+           spec.BITS
+           spec.toNat
+           thirtyTwo
+           two
+
+       }.
+
+Theorem cork_uncork_high :
+  forall c,
+    ConnectionRecordPP0.corked c = bvNat 2 0 ->
+    s2nCork c = bvNat 2 1.
+Proof.
+  (* use lifted *)
+Qed.
+
+Theorem cork_uncork : forall c,
+    ConnectionRecordPP0.corked c = bvNat 2 0 ->
+    uncork (cork c) = c.
+Proof.
+  intros [] H.
+  simpl in H.
+  unfold cork, uncork.
+  simpl.
+  f_equal.
+  unfold s2nCork.
+  simpl.
+  unfold s2nUncork.
+  simpl.
+  unfold ecPlus. unfold Notation.Rget. simpl.
+  unfold ecMinus. unfold Notation.Rget. simpl.
+  subst corked.
+  unfold joinLSB.
+  simpl.
+  unfold bvAdd.
+  simpl.
+  unfold bvToBITS.
+  simpl.
+  unfold bvToNatFolder.
+  simpl.
+  compute.
+  apply val_inj.
+Qed.
+
+Theorem test : forall c,
+    c {| corked := _; |} = c.
+
+    S2N'.s2n_cork (S2N'.s2n_uncork c) = c.
+
+Stop.
+
+(* ACTIVE_MESSAGE is too complex *)
+
+Print S2NPP.S2N'.ACTIVE_MESSAGE.
+
+Check (S2NPP.S2N'.ACTIVE_MESSAGE : ConnectionPP.connection -> seq 32 bool).
+
+Lift HandshakePP.handshake
+     HandshakeRecordPP.Handshake
+  in S2N'.ACTIVE_MESSAGE
+  as ActiveMessage0.
+
+Lift ConnectionPPconnection
+     ConnectionRecordPP1.Connection
+  in ActiveMessage0
+  as ActiveMessage.
+
+Lift connectionPP ConnectionPP.Connection
+  in ActiveMessage0
+  as ActiveMessage.
+
+Lift HandshakePP.handshake
+     HandshakePP.Handshake
+  in S2N'.advance_message
+  as advanceMessage0.
+
+(* This one does not terminate. *)
+Lift connectionPP ConnectionPP.Connection
+  in advanceMessage0
+  as advanceMessage.
+
+Definition myHandshake : HandshakePP.Handshake :=
+  HandshakePP.MkHandshake
+    (bvNat _ 0)
+    (bvNat _ 0)
+.
+
+Definition myConnection : ConnectionPP.Connection :=
+  ConnectionPP.MkConnection
+    (false)
+    (bvNat _ 0)
+    (bvNat _ 0)
+    (myHandshake)
+    (false)
+    (false)
+    (bvNat _ 0)
+    (false)
+    (false)
+.
