coq/handwritten/Lift/Lift/HandshakeLift.v
@@ -1,0 +1,96 @@
+From Bits Require Import spec.
+
+From Coq Require Import String.
+From Coq Require Import Vectors.Vector.
+
+From CryptolToCoq Require Import CryptolPrimitivesForSAWCore.
+From CryptolToCoq Require Import CryptolPrimitivesForSAWCoreExtra.
+From CryptolToCoq Require Import SAWCorePrelude.
+From CryptolToCoq Require Import SAWCorePrelude_proofs.
+From CryptolToCoq Require Import SAWCoreScaffolding.
+From CryptolToCoq Require Import SAWCoreVectorsAsCoqVectors.
+
+From Lift Require Import Preprocess.S2NPP.
+From Lift Require Import Preprocess.HandshakePP.
+
+From Ornamental Require Import Ornaments.
+
+From S2N Require Import S2N.
+
+Set DEVOID search prove equivalence.
+Set DEVOID lift type.
+
+Set Preprocess default opaque.
+
+Import CryptolPrimitives.
+
+Print HandshakePP.handshake.
+
+Module HandshakeRecord.
+
+  (** We can define more convenient types for [handshake] and [connection] in Coq.
+Ideally, we'd like the translation to generate those, but in its current state,
+it goes through an intermediate language that does not support records and
+record types.
+   *)
+  Record Handshake :=
+    MkHandshake
+      {
+        handshakeType : seq 32 bool;
+        messageNumber : seq 32 bool;
+      }.
+
+  Scheme Induction for Handshake Sort Prop.
+  Scheme Induction for Handshake Sort Type.
+  Scheme Induction for Handshake Sort Set.
+
+  Definition get_handshake_type (h : HandshakePP.handshake) : seq 32 bool :=
+    fst h.
+
+  Definition get_message_number (h : HandshakePP.handshake) : seq 32 bool :=
+    snd h.
+
+End HandshakeRecord.
+
+Preprocess Module HandshakeRecord as HandshakeRecordPP { opaque ecAt }.
+
+Lift HandshakePP.handshake
+     HandshakeRecordPP.Handshake
+  in HandshakeRecordPP.get_handshake_type
+  as getHandshakeType.
+
+Lift HandshakePP.handshake
+     HandshakeRecordPP.Handshake
+  in HandshakeRecordPP.get_message_number
+  as getMessageNumber.
+
+Lift HandshakePP.handshake
+     HandshakeRecordPP.Handshake
+  in S2N'.ACTIVE_MESSAGE
+  as ActiveMessage0 { opaque S2N'.handshakes }.
+
+Lift HandshakePP.handshake
+     HandshakeRecordPP.Handshake
+  in S2N'.valid_handshake
+  as validHandshake0
+{ opaque
+PArithSeqBool
+PCmpSeq
+PCmpSeqBool
+PCmpSeqBool
+PLiteralSeqBool
+PZeroSeq
+PZeroSeqBool
+S2N'.and
+S2N'.handshakes_fn
+S2N'.length
+ecAt
+ecGt
+ecLt
+ecMinus
+ecNotEq
+ecNumber
+ecPlus
+ecZero
+seq
+}.
