coq/handwritten/Lift/Preprocess/HandshakePP.v
@@ -1,0 +1,45 @@
+From CryptolToCoq Require Import CryptolPrimitivesForSAWCore.
+From CryptolToCoq Require Import SAWCoreScaffolding.
+From CryptolToCoq Require Import SAWCorePrelude.
+
+From S2N Require Import S2N.
+From S2N Require Import Translation.Handshake.
+
+From mathcomp Require Import eqtype.
+From mathcomp Require Import fintype.
+From mathcomp Require Import ssrnat.
+From mathcomp Require Import seq.
+From mathcomp Require Import tuple.
+
+Scheme Minimality for tuple.tuple_of Sort Prop.
+Scheme Induction  for tuple.tuple_of Sort Set.
+Scheme Induction  for tuple.tuple_of Sort Type.
+
+Scheme Minimality for eqtype.Equality.type Sort Prop.
+Scheme Induction  for eqtype.Equality.type Sort Set.
+Scheme Induction  for eqtype.Equality.type Sort Type.
+
+Scheme Minimality for eqtype.Equality.mixin_of Sort Prop.
+Scheme Induction  for eqtype.Equality.mixin_of Sort Set.
+Scheme Induction  for eqtype.Equality.mixin_of Sort Type.
+
+Scheme Induction for eqtype.Sub_spec Sort Prop.
+Scheme Induction for eqtype.Sub_spec Sort Set.
+Scheme Induction for eqtype.Sub_spec Sort Type.
+
+Scheme Induction for eqtype.insub_spec Sort Prop.
+Scheme Induction for eqtype.insub_spec Sort Set.
+Scheme Induction for eqtype.insub_spec Sort Type.
+
+Scheme Induction for eqtype.subType Sort Prop.
+Scheme Induction for eqtype.subType Sort Set.
+Scheme Induction for eqtype.subType Sort Type.
+
+From Ornamental Require Import Ornaments.
+
+Set DEVOID search prove equivalence. (* <-- Correctness proofs for search *)
+Set DEVOID lift type. (* <-- Prettier types than the ones Coq infers *)
+
+Set Preprocess default opaque.
+
+Preprocess Module Handshake as HandshakePP.
